Lp2lc/Active/package.lean
@@ -1,5 +1,4 @@
 
 -- STLC module exports Def and Example
-import «Lp2lc».Active.STLC.Def
 import «Lp2lc».Active.STLC.Proof
 import «Lp2lc».Active.STLC.SI.Proof
